ne coinductive dostep with single output

DataflowToObc/Correctness.v
@@ -1770,6 +1770,225 @@ for all [Is_free_exp x e]. *)
             now injection 1; intro; subst.
     Qed.
 
+    Inductive event := Read : list const -> event | Write : value -> event.
+    CoInductive trace := Ev : event -> trace -> trace.
+
+    Definition ev t := match t with Ev a _ => a end.
+    Definition tl t := match t with Ev _ b => b end.
+
+
+    Lemma unroll_event:
+      forall (t: trace), t = Ev (ev t) (tl t).
+    Proof.
+    intros. destruct t; auto. 
+    Qed.
+    
+    Ltac sunroll x := rewrite (unroll_event x); simpl.
+
+
+    CoInductive bisim: trace -> trace -> Prop :=
+    | bisim_cons: forall s1 s2,
+        ev s1 = ev s2 -> bisim (tl s1) (tl s2) -> bisim s1 s2.
+
+    Remark bisim_refl: forall (t: trace), bisim t t.
+    Proof.
+    cofix COINDHYP; intros; constructor; auto.
+    Qed.
+
+    Remark bisim_sym: forall (s1 s2: trace), bisim s1 s2 -> bisim s2 s1.
+    Proof.
+    cofix COINDHYP; intros. inv H; constructor; auto.
+    Qed.
+
+    Remark bisim_trans:
+      forall (s1 s2 s3: trace), bisim s1 s2 -> bisim s2 s3 -> bisim s1 s3.
+    Proof.
+    cofix COINDHYP; intros. inv H; inv H0; constructor; eauto. congruence.
+    Qed.
+
+    Require Import Setoid.
+
+    Add Parametric Relation : trace bisim
+        reflexivity proved by bisim_refl
+        symmetry proved by bisim_sym
+        transitivity proved by bisim_trans
+          as bisim_R.
+
+    Add Parametric Morphism : Ev 
+        with signature eq ==> bisim ==> bisim
+          as Ev_M.
+    Proof. intros; constructor; auto. Qed.
+    
+    Add Parametric Morphism : ev 
+        with signature bisim ==> eq
+          as ev_M.
+    Proof. intros. inv H; auto. Qed.
+
+    Add Parametric Morphism : tl
+        with signature bisim ==> bisim
+          as tl_M.
+    Proof. intros. inv H; auto. Qed.
+
+    Notation "A == B" := (bisim A B) (at level 70, no associativity).
+
+
+    CoFixpoint mk_trace' (n : nat) 
+      := Ev (Read (css n)) 
+              (Ev (Write (ys n))
+                    (mk_trace' (S n))).
+    
+    Definition mk_trace := mk_trace' 0.    
+
+    Definition unroll_trace : 
+      forall n, mk_trace' n = Ev (Read (css n)) 
+                             (Ev (Write (ys n))
+                                 (mk_trace' (S n))).
+    Proof. 
+    intros.
+    sunroll (mk_trace' n). reflexivity.
+    Qed.
+
+    CoInductive dostep' P : nat -> heap -> stack -> trace -> Prop
+      := Step : forall n css ys menv0 env0 menv1 env1 t,
+          let cs := map Const css in
+          stmt_eval P menv0 env0 (Call [r] main obj step cs) (menv1, env1) ->
+          (exists y, ys = present y /\ PM.find r env1 = Some y) -> 
+          dostep' P (S n) menv1 env1 t ->
+          dostep' P n menv0 env0 (Ev (Read css) (Ev (Write ys) t)).
+
+    Section Dostep'_coind.
+
+    Variable P : program.
+    Variable R : nat -> heap -> stack -> trace -> Prop.
+
+    Hypothesis StepCase: forall n menv0 env0 t,
+      R n menv0 env0 t ->
+      exists css ys t' menv1 env1,
+        let cs := map Const css in
+          stmt_eval P menv0 env0 (Call [r] main obj step cs) (menv1, env1) 
+        /\ (exists y, ys = present y /\ PM.find r env1 = Some y)
+        /\ R (S n) menv1 env1 t'
+        /\ t = (Ev (Read css) (Ev (Write ys) t')).
+
+    Lemma dostep'_coind : forall n menv env t,
+        R n menv env t -> dostep' P n menv env t.
+    Proof.
+    cofix COINDHYP.
+    intros.
+    edestruct (StepCase _ _ _ _ H).
+    simpl in H0.
+    decompose record H0.
+    rewrite H6.
+    econstructor; eauto.
+    Qed.
+    
+    End Dostep'_coind.
+
+    Lemma dostep'_correct: 
+      forall M,
+        let P := translate G in
+        msem_node G main xss M ys ->
+        exists menv0 env0,
+            stmt_eval (translate G) hempty sempty (Call [] main obj reset []) (menv0, env0) 
+          /\ dostep' (translate G) 0 menv0 env0 mk_trace.
+    Proof.
+    intros M Hdef Hmsem. 
+    assert (exists menv' env',
+               stmt_eval (translate G) hempty sempty
+                         (Call [] main obj reset []) (menv', env')
+               /\ (exists omenv0,   mfind_inst obj menv' = Some omenv0
+                            /\ Memory_Corres G 0 main M omenv0))
+      as (menv0 & env0 & Hstmtr & (omenv0 & Hmf0 & Hmc0)).
+    {
+      pose proof (is_node_reset_correct _ _ Hwdef _ _ _ Hmsem hempty) as Hrst.
+      destruct Hrst as (omenv' & Hcall & Hcor).
+        intros. do 2 eexists.
+        split.
+      - econstructor; eauto.
+        rewrite mfind_inst_empty. eassumption.
+      - exists omenv'.
+        split; auto.
+        apply mfind_inst_gss.
+    }
+    
+    exists menv0, env0; split; auto.
+    set (R := fun n (menv: heap) (env: stack) (t: trace) => 
+                exists omenv,   mfind_inst obj menv = Some omenv
+                         /\ Memory_Corres G n main M omenv
+                         /\ t = mk_trace' n).
+    apply dostep'_coind with (R := R).
+    2: unfold R; eexists; eauto.
+    intros. unfold R in H. 
+    destruct H as (? & ? & ? & ?).
+    rewrite unroll_trace in H1.
+
+    exists (css n).
+    exists (ys n).
+    exists (mk_trace' (S n)).
+    
+    set (ciSn := css n).
+
+    assert (HpresN: xss n = map present (map sem_const ciSn))
+      by (subst xss; unfold present_list; rewrite map_map; eauto).
+
+    assert (exists coSn, ys n = present coSn) as [coSn Hys] by admit.
+    (* { *)
+    (*   inversion_clear Hmsem as *)
+    (*       [? ? ? ? ? ? ? ? ? ? ? ? ? ? ? Hbk Hfind *)
+    (*          (H' & Hsem_in & Hsem_out & Hsamexs & Hsameys & Habs & Hsem_eqns)]. *)
+      
+    (*   assert (Hlen: 0 < length ciSn). *)
+    (*   { *)
+    (*     assert (length ciSn = length (xss n)) as -> *)
+    (*         by now rewrite HpresN, 2 map_length. *)
+        
+    (*     assert (length (map fst i) = length (xss n)) as <- *)
+    (*         by now eapply Forall2_length; *)
+    (*       specialize (Hsem_in n); simpl in Hsem_in; *)
+    (*         eauto. *)
+        
+    (*     now rewrite map_length. *)
+    (*   } *)
+      
+    (*   assert (present_list (yss n)). *)
+    (*   { *)
+    (*         edestruct Hsameys as [Habs_ys|]; eauto. *)
+    (*         apply Habs in Habs_ys. rewrite HpresN in Habs_ys. *)
+    (*         destruct ciSn; try now inv Hlen. simpl in Habs_ys. *)
+    (*         inv Habs_ys. discriminate. *)
+    (*   } *)
+      
+    (*   now apply present_list_spec. *)
+    (* } *)
+    
+    assert (exists menvN' envN',
+               stmt_eval (translate G) menv1 env1
+                         (Call [r] main obj step (map Const ciSn))
+                         (menvN', envN')
+               /\ (exists omenvsN, mfind_inst obj menvN' = Some omenvsN
+                             /\ Memory_Corres G (S n) main M omenvsN)
+               /\ PM.find r envN' = Some coSn)
+      as (menvSn & envSn & Hstmt & (omenvSn & Hmfind & Hmc) & Hout).
+    { 
+      edestruct is_node_correct as (omenvsN & Hstmt & HmcSn); eauto.
+      do 2 eexists.
+      repeat split.
+      - econstructor; eauto.
+        2:rewrite H; now eapply Hstmt.
+        clear Hstmt HpresN.
+        induction ciSn; simpl; auto.
+      - exists omenvsN. split; auto.
+        now rewrite mfind_inst_gss.
+      - unfold adds; simpl. rewrite PM.gss; auto.
+    }
+
+    exists menvSn, envSn.
+    repeat split; auto.
+    - rewrite Hys; eauto.
+    - unfold R.
+      exists omenvSn. repeat split; auto.
+    Qed.
+
     Theorem is_event_loop_correct:
       (* =translate_correct= *)
       sem_node G main xss ys ->
